update regions

spec/flat.s.dfy
@@ -1,340 +1,349 @@
 include "bvop/bv_op.s.dfy"
+include "bvop/bv16_op.s.dfy"
+include "bvop/bv32_op.s.dfy"
+include "bvop/bv256_op.s.dfy"
 // include "crypto/pow2.s.dfy"
 
-module SetOfMaps {
-    predicate {:opaque} keysDisjoint<K, V>(ms: set<map<K, V>>)
-    {
-        forall m1, m2 | (m1 in ms && m2 in ms && m1 != m2)
-            :: m1.Keys !! m2.Keys
-    }
-
-    function flattenMaps<K,V>(ms: set<map<K, V>>): map<K, V>
-        requires keysDisjoint(ms)
-    {
-        reveal keysDisjoint();
-        map m, k | (m in ms && k in m) :: k := m[k]
-    }
-
-    lemma flattenMapsElemSufLemma<K,V>(ms: set<map<K, V>>, k: K)
-        returns (m: map<K, V>)
-        requires keysDisjoint(ms)
-        requires k in flattenMaps(ms)
-        ensures m in ms && k in m
-        ensures m[k] == flattenMaps(ms)[k]
-    {
-        reveal keysDisjoint();
-        m :| m in ms && k in m;
-        assert flattenMaps(ms)[k] == m[k];
-    }
-
-    lemma flattenMapsElemNecLemma<K,V>(ms: set<map<K, V>>, m: map<K, V>, k: K)
-        requires keysDisjoint(ms)
-        requires m in ms && k in m
-        ensures k in flattenMaps(ms)
-        ensures m[k] == flattenMaps(ms)[k]
-    {
-    }
-
-    lemma flattenMapsUpdateLemma<K,V>(ms: set<map<K, V>>, ms': set<map<K, V>>,
-        n: map<K,V>, n': map<K,V>, k: K, v: V)
-        requires keysDisjoint(ms)
-        requires keysDisjoint(ms')
-        requires n in ms
-        requires n' in ms'
-        requires ms' == ms - {n} + {n'}
-        requires k in n
-        requires k in n'
-        requires n'[k] == v
-        requires n' == n[k := v]
-        ensures flattenMaps(ms') == flattenMaps(ms)[k := v]
-    {
-        reveal keysDisjoint();
-        var m := flattenMaps(ms);
-        var m' := flattenMaps(ms');
-
-        forall key | key in m'
-            ensures key in m
-            ensures key != k ==> m[key] == m'[key]
-            ensures key == k ==> m[key] == n'[key]
-        {
-            var _ := flattenMapsElemSufLemma(ms, key);
-            var _ := flattenMapsElemSufLemma(ms', key);
-        }
-
-        assert m' == m[k := v];
-    }
-}
-
-module flat {
+abstract module flat_mem_s(BV: bv_op_s) {
     import opened integers
+    import BS = BV.BVSEQ
+
     import Power
+    import Mul
 
-    import opened SetOfMaps
+    // how many bytes in the word
+    const WORD_BYTES: nat
 
-    datatype flat_t = flat_t(raw: map<nat, uint8>, max: nat)
+    // how many words in the memory
+    const MAX_WORDS: nat
+
+    function MAX_BYTES(): nat 
     {
-        predicate {:opaque} inv()
-        {
-            && max != 0
-            && (forall addr | addr in raw :: addr < max)
-        }
-
-        function method do_read(ptr: nat): uint8
-            requires inv()
-        {
-            if ptr in raw then raw[ptr] else 0 
-        }
-
-        function method do_write(ptr: nat, value: uint8): flat_t
-            requires inv()
-            requires ptr < max;
-            ensures inv()
-        {
-            reveal inv();
-            var raw' := if ptr in raw then raw[ptr := value] else raw;
-            this.(raw := raw')
-        }
+        Mul.LemmaMulNonnegative(WORD_BYTES, MAX_WORDS);
+        WORD_BYTES * MAX_WORDS
     }
 
-    datatype regions_t = regions_t(regions: map<nat, seq<uint8>>, max: nat)
+    // obligation
+    lemma word_size_lemma()
+        ensures WORD_BYTES != 0
+        ensures Power.Pow(256, WORD_BYTES) == BS.BASE()
+
+    // points to a word with aligment
+    predicate ptr_aligned(ptr: nat)
     {
-        predicate valid_region_index(base: nat, i: nat)
+        word_size_lemma();
+        && ptr % WORD_BYTES == 0
+        && ptr + WORD_BYTES <= MAX_BYTES()
+    }
+
+    // aligned adddresses only
+    type aptr = i :nat | ptr_aligned(i) witness *
+
+    const STACK_MAX_WORDS: nat
+
+    const STACK_BOT: aptr
+
+    datatype mem_t = mem_cons(
+        // the flat memory, 
+        flat: map<aptr, BS.uint>,
+        // ghost state about memory structure
+        ghost split: map<aptr, nat>)
+    {
+        // single word read/write
+
+        function method read_word(ptr: aptr): BS.uint
         {
-            && base in regions
-            && 0 <= i < |regions[base]|
+            if ptr in flat then flat[ptr] else 0 
         }
 
-        function do_read_(base: nat, i: nat): uint8
-            requires valid_region_index(base, i)
+        function method write_word(ptr: aptr, value: BS.uint): mem_t
         {
-            regions[base][i]
+            var flat' := if ptr in flat then flat[ptr := value] else flat;
+            mem_cons(flat', split)
         }
 
-        function do_write_(base: nat, i: nat, value: uint8): regions_t
-            requires valid_region_index(base, i)
+        // multi words read/write
+
+        predicate valid_multi_word(ptr: aptr, count: nat)
         {
-            var region' := regions[base][i := value];
-            var regions' := regions[base := region'];
-            this.(regions := regions')
+            ptr + count * WORD_BYTES <= MAX_BYTES()
         }
 
-        predicate region_inv(base: nat)
-            requires base in regions
+        // assumptions about the initial memory state
+
+        predicate region_valid(base: nat, len: nat)
         {
-            && var len := |regions[base]|;
-            && len != 0
-            && base + len < max
-            && (forall i | 1 <= i < len ::
-                (base + i) !in regions)
+            // the addresses are all mapped
+            && (forall i | 0 <= i < len :: 
+                base + i * WORD_BYTES in flat)
+            // the addresses are all bounded
+            && base + len * WORD_BYTES < MAX_BYTES()
         }
 
-        predicate {:opaque} inv()
+        predicate inv()
         {
-            && max != 0
-            && (forall base | base in regions ::
-                region_inv(base))
-        }
-
-        function region_as_raw(base: nat): (f: map<nat, uint8>)
-            requires base in regions
-        {
-            map k | base <= k < base + |regions[base]| ::
-                do_read_(base, k - base)
-        }
-
-        function regions_as_raws_(): set<map<nat, uint8>>
-        {
-            set base | base in regions :: region_as_raw(base)
-        }
-
-        lemma region_indices_disjoint_lemma(base1: nat, i: nat, base2: nat, j: nat)
-            requires inv()
-            requires valid_region_index(base1, i);
-            requires valid_region_index(base2, j);
-            requires base1 != base2
-            ensures base1 + i != base2 + j
-        {
-            assert region_inv(base1) && region_inv(base2) by {
-                reveal inv();
-            }
-
-            if base1 + i == base2 + j {
-                var buff1 := regions[base1];
-                var buff2 := regions[base2];
-
-                if base1 > base2 {
-                    assert region_inv(base2);
-                    var k := j - i;
-                    assert base1 == base2 + k;
-                    assert 0 <= k < |buff2|;
-                    assert base1 !in regions;
-                    assert false;
-                } else {
-                    assert region_inv(base1);
-                    var k := i - j;
-                    assert base2 == base1 + k;
-                    assert 0 <= k < |buff1|;
-                    assert base2 !in regions;
-                    assert false;
-                }
-            }
-        }
-
-        predicate disjoint_regions(base1: nat, base2: nat)
-        {
-            && base1 in regions
-            && base2 in regions
-            && base1 != base2
-        }
-
-        lemma region_properties_lemma()
-            requires inv()
-            ensures keysDisjoint(regions_as_raws_())
-            ensures forall k, m | (m in regions_as_raws_() && k in m) :: k < max
-        {
-            reveal keysDisjoint();
-            forall base1 , base2 | disjoint_regions(base1, base2)
-                ensures region_as_raw(base1).Keys !! region_as_raw(base2).Keys
-            {
-                var m1 := region_as_raw(base1).Keys;
-                var m2 := region_as_raw(base2).Keys;
-
-                if !(m1 !! m2) {
-                    var k :| k in m1 && k in m2;
-                    var i :| k == i + base1;
-                    var j :| k == j + base2;
-                    region_indices_disjoint_lemma(base1, i, base2, j);
-                }
-            }
-            reveal inv();
-        }
-
-        function regions_as_raws(): (rs: set<map<nat, uint8>>)
-            requires inv();
-            ensures keysDisjoint(rs)
-        {
-            region_properties_lemma();
-            regions_as_raws_()
-        }
-
-        function {:opaque} as_flat(): (f: flat_t)
-            requires inv()
-            ensures f.inv()
-            ensures f.max == max
-        {
-            var rs := flattenMaps(regions_as_raws());
-            var f := flat_t(rs, max);
-            assert f.inv() by {reveal inv(); reveal f.inv();}
-            f
-        }
-
-        lemma valid_region_index_bound_lemma(base: nat, i: nat)
-            requires inv()
-            requires valid_region_index(base, i)
-            ensures base + i < max
-        {
-            reveal inv();
-        }
-
-        lemma do_read_lemma(base: nat, i: nat)
-            requires inv()
-            requires valid_region_index(base, i)
-            ensures do_read_(base, i) == as_flat().do_read(base + i)
-        {
-            reveal keysDisjoint();
-            var raw := as_flat().raw;
-            var raws := regions_as_raws();
-            valid_region_index_bound_lemma(base, i);
-            var rraw := region_as_raw(base);
-
-            flattenMapsElemNecLemma(raws, rraw, base + i);
-            reveal as_flat();
-        }
-
-        function do_read(base: nat, i: nat): (v: uint8)
-            requires inv()
-            requires valid_region_index(base, i)
-            ensures v == as_flat().do_read(base + i)
-        {
-            do_read_lemma(base, i);
-            do_read_(base, i)
-        }
-
-        lemma do_write_lemma(base: nat, i: nat, value: uint8)
-            requires inv()
-            requires valid_region_index(base, i)
-            ensures var that := do_write_(base, i, value);
-                && that.inv()
-                && base + i < max
-                && that.as_flat() == as_flat().do_write(base + i, value)
-        {
-            var that := do_write_(base, i, value);
-
-            assert that.inv() by {
-                reveal inv();
-
-                forall base1 | base1 in that.regions
-                    ensures that.region_inv(base)
-                {
-                    if base1 != base {
-                        assert that.regions[base1] == regions[base1];
-                    } else {
-                        var region' := regions[base][i := value];
-                        assert that.regions[base] == region';
-                    }
-                }
-            }
-
-            var raws := regions_as_raws();
-            var raw := flattenMaps(raws);
-            var raws' := that.regions_as_raws();
-            var raw' := flattenMaps(raws');
-            var ptr :nat := base + i;
-
-            var rr := region_as_raw(base);
-            var rr' := that.region_as_raw(base);
-
-            assert raws' == raws - {rr} + {rr'} 
-                && rr in raws 
-                && rr' in raws' 
-                && rr' == rr[ptr := value] by {
-                forall base' | base' in that.regions
-                    ensures base' in regions;
-                    ensures base' != base ==>
-                        that.region_as_raw(base') == region_as_raw(base');
-                    ensures base' == base ==>
-                        that.region_as_raw(base) == rr[i + base := value];
-                {
-                    var region := regions[base'];
-                    var region' := that.regions[base'];
-                    if base' != base {
-                        assert region' == region;
-                        assert that.region_as_raw(base') == region_as_raw(base');
-                    } else {
-                        assert region' == region[i := value];
-                        assert rr' == rr[i + base := value];
-                    }
-                }
-            }
-
-            assert raw' == raw[ptr := value] by {
-                flattenMapsUpdateLemma(raws, raws', rr, rr', ptr, value);
-            }
-
-            valid_region_index_bound_lemma(base, i);
-
-            assert raw' == that.as_flat().raw by {
-                reveal that.as_flat();
-            }
-
-            assert raw == as_flat().raw by {
-                reveal as_flat();
-            }
-
-            assert that.as_flat() == as_flat().do_write(ptr, value);
+            // stack region
+            && STACK_BOT in split
+            && split[STACK_BOT] == STACK_MAX_WORDS
+            // all the regions are valid
+            && (forall base | base in split ::
+                region_valid(base, split[base]))
+            // regions are disjoint
+            && (forall b1, b2 | (b1 in split && b2 in split && b1 != b2) ::
+                    (b1 >= b2 + split[b2] || b2 >= b1 + split[b1]))
         }
     }
 }
+
+
+    // datatype regions_t = regions_t(regions:, max: nat)
+    // {
+    //     predicate region_inv(base: nat)
+    //         requires base in regions
+    //     {
+    //         && var len := |regions[base]|;
+    //         && len != 0
+    //         && base + len < max
+    //         && (forall i | 1 <= i < len ::
+    //             (base + i) !in regions)
+    //     }
+
+    //     predicate {:opaque} inv()
+    //     {
+    //         && max != 0
+    //         && (forall base | base in regions ::
+    //             region_inv(base))
+    //     }
+
+    //     function region_as_raw(base: nat): (f: map<nat, uint8>)
+    //         requires base in regions
+    //     {
+    //         map k | base <= k < base + |regions[base]| ::
+    //             do_read_(base, k - base)
+    //     }
+
+    //     function regions_as_raws_(): set<map<nat, uint8>>
+    //     {
+    //         set base | base in regions :: region_as_raw(base)
+    //     }
+
+    //     lemma region_indices_disjoint_lemma(base1: nat, i: nat, base2: nat, j: nat)
+    //         requires inv()
+    //         requires region_index_valid(base1, i);
+    //         requires region_index_valid(base2, j);
+    //         requires base1 != base2
+    //         ensures base1 + i != base2 + j
+    //     {
+    //         assert region_inv(base1) && region_inv(base2) by {
+    //             reveal inv();
+    //         }
+
+    //         if base1 + i == base2 + j {
+    //             var buff1 := regions[base1];
+    //             var buff2 := regions[base2];
+
+    //             if base1 > base2 {
+    //                 assert region_inv(base2);
+    //                 var k := j - i;
+    //                 assert base1 == base2 + k;
+    //                 assert 0 <= k < |buff2|;
+    //                 assert base1 !in regions;
+    //                 assert false;
+    //             } else {
+    //                 assert region_inv(base1);
+    //                 var k := i - j;
+    //                 assert base2 == base1 + k;
+    //                 assert 0 <= k < |buff1|;
+    //                 assert base2 !in regions;
+    //                 assert false;
+    //             }
+    //         }
+    //     }
+
+    //     predicate disjoint_regions(base1: nat, base2: nat)
+    //     {
+    //         && base1 in regions
+    //         && base2 in regions
+    //         && base1 != base2
+    //     }
+
+    //     lemma region_properties_lemma()
+    //         requires inv()
+    //         ensures keysDisjoint(regions_as_raws_())
+    //         ensures forall k, m | (m in regions_as_raws_() && k in m) :: k < max
+    //     {
+    //         reveal keysDisjoint();
+    //         forall base1 , base2 | disjoint_regions(base1, base2)
+    //             ensures region_as_raw(base1).Keys !! region_as_raw(base2).Keys
+    //         {
+    //             var m1 := region_as_raw(base1).Keys;
+    //             var m2 := region_as_raw(base2).Keys;
+
+    //             if !(m1 !! m2) {
+    //                 var k :| k in m1 && k in m2;
+    //                 var i :| k == i + base1;
+    //                 var j :| k == j + base2;
+    //                 region_indices_disjoint_lemma(base1, i, base2, j);
+    //             }
+    //         }
+    //         reveal inv();
+    //     }
+
+    //     function regions_as_raws(): (rs: set<map<nat, uint8>>)
+    //         requires inv();
+    //         ensures keysDisjoint(rs)
+    //     {
+    //         region_properties_lemma();
+    //         regions_as_raws_()
+    //     }
+
+    //     function {:opaque} as_flat(): (f: flat_t)
+    //         requires inv()
+    //         ensures f.inv()
+    //         ensures f.max == max
+    //     {
+    //         var rs := flattenMaps(regions_as_raws());
+    //         var f := flat_t(rs, max);
+    //         assert f.inv() by {reveal inv(); reveal f.inv();}
+    //         f
+    //     }
+
+    //     lemma region_index_valid_bound_lemma(base: nat, i: nat)
+    //         requires inv()
+    //         requires region_index_valid(base, i)
+    //         ensures base + i < max
+    //     {
+    //         reveal inv();
+    //     }
+
+    //     lemma do_read_lemma(base: nat, i: nat)
+    //         requires inv()
+    //         requires region_index_valid(base, i)
+    //         ensures do_read_(base, i) == as_flat().do_read(base + i)
+    //     {
+    //         reveal keysDisjoint();
+    //         var raw := as_flat().raw;
+    //         var raws := regions_as_raws();
+    //         region_index_valid_bound_lemma(base, i);
+    //         var rraw := region_as_raw(base);
+
+    //         flattenMapsElemNecLemma(raws, rraw, base + i);
+    //         reveal as_flat();
+    //     }
+
+    //     function do_read(base: nat, i: nat): (v: uint8)
+    //         requires inv()
+    //         requires region_index_valid(base, i)
+    //         ensures v == as_flat().do_read(base + i)
+    //     {
+    //         do_read_lemma(base, i);
+    //         do_read_(base, i)
+    //     }
+
+    //     lemma do_write_lemma(base: nat, i: nat, value: uint8)
+    //         requires inv()
+    //         requires region_index_valid(base, i)
+    //         ensures var that := do_write_(base, i, value);
+    //             && that.inv()
+    //             && base + i < max
+    //             && that.as_flat() == as_flat().do_write(base + i, value)
+    //     {
+    //         var that := do_write_(base, i, value);
+
+    //         assert that.inv() by {
+    //             reveal inv();
+
+    //             forall base1 | base1 in that.regions
+    //                 ensures that.region_inv(base)
+    //             {
+    //                 if base1 != base {
+    //                     assert that.regions[base1] == regions[base1];
+    //                 } else {
+    //                     var region' := regions[base][i := value];
+    //                     assert that.regions[base] == region';
+    //                 }
+    //             }
+    //         }
+
+    //         var raws := regions_as_raws();
+    //         var raw := flattenMaps(raws);
+    //         var raws' := that.regions_as_raws();
+    //         var raw' := flattenMaps(raws');
+    //         var ptr :nat := base + i;
+
+    //         var rr := region_as_raw(base);
+    //         var rr' := that.region_as_raw(base);
+
+    //         assert raws' == raws - {rr} + {rr'} 
+    //             && rr in raws 
+    //             && rr' in raws' 
+    //             && rr' == rr[ptr := value] by {
+    //             forall base' | base' in that.regions
+    //                 ensures base' in regions;
+    //                 ensures base' != base ==>
+    //                     that.region_as_raw(base') == region_as_raw(base');
+    //                 ensures base' == base ==>
+    //                     that.region_as_raw(base) == rr[i + base := value];
+    //             {
+    //                 var region := regions[base'];
+    //                 var region' := that.regions[base'];
+    //                 if base' != base {
+    //                     assert region' == region;
+    //                     assert that.region_as_raw(base') == region_as_raw(base');
+    //                 } else {
+    //                     assert region' == region[i := value];
+    //                     assert rr' == rr[i + base := value];
+    //                 }
+    //             }
+    //         }
+
+    //         assert raw' == raw[ptr := value] by {
+    //             flattenMapsUpdateLemma(raws, raws', rr, rr', ptr, value);
+    //         }
+
+    //         region_index_valid_bound_lemma(base, i);
+
+    //         assert raw' == that.as_flat().raw by {
+    //             reveal that.as_flat();
+    //         }
+
+    //         assert raw == as_flat().raw by {
+    //             reveal as_flat();
+    //         }
+
+    //         assert that.as_flat() == as_flat().do_write(ptr, value);
+    //     }
+    // }
+
+// module regioned_mem_s(BV: bv_op_s, LM: linear_mem_s(BV)) 
+// {
+//     type uint = BV.BVSEQ.uint
+
+//     type regions_t =  map<nat, seq<uint>>
+
+
+//     function do_read_(regions: regions_t, base: nat, i: nat): uint
+//         requires region_index_valid(regions, base, i)
+//     {
+//         regions[base][i]
+//     }
+
+//     function do_write_(regions: regions_t, base: nat, i: nat, value: uint): regions_t
+//         requires region_index_valid(regions, base, i)
+//     {
+//         var region' := regions[base][i := value];
+//         regions[base := region']
+//     }
+
+//     function as_linear(regions: regions_t): LM.mem_t
+// }
+
+
+
+    // datatype mem_t = mem_cons(heap: ,stack: )
+
+
+
         // lemma regions_disjoint_lemma(base1: nat, base2: nat)
         //     requires inv()
         //     requires disjoint_regions(base1, base2)
@@ -355,7 +364,7 @@ module flat {
         //     returns (base: nat, i: nat)
         //     requires inv()
         //     requires addr in regions_as_raw()
-        //     ensures valid_region_index(base, i)
+        //     ensures region_index_valid(base, i)
         //     ensures addr == base + i 
         //     ensures regions_as_raw()[addr] == read_region_index(base, i)
         // {
@@ -376,12 +385,12 @@ module flat {
         //     requires base in regions
         //     requires addr in region_as_raw(base)
         //     ensures addr >= base
-        //     ensures valid_region_index(base, addr-base)
+        //     ensures region_index_valid(base, addr-base)
         //     ensures addr == i + base
         //     ensures region_as_raw(base)[addr] == regions[base][i]
         // {
         //     assert base <= addr < base + |regions[base]|;
         //     i := addr - base;
-        //     assert valid_region_index(base, i) && base + i == addr;
+        //     assert region_index_valid(base, i) && base + i == addr;
         // }
 
