spec/regions.i.dfy
@@ -1,0 +1,411 @@
+include "flat.s.dfy"
+
+abstract module regions_mem_i(BV: bv_op_s) {
+    import opened integers
+    import FM = flat_mem_s(BV)
+    import BS = FM.BS
+
+    import Mul
+
+    type regions_t = map<nat, seq<BS.uint>>
+
+    predicate region_index_valid(regions: regions_t, base: nat, i: nat)
+    {
+        && base in regions
+        && 0 <= i < |regions[base]|
+    }
+
+    function read_region(regions: regions_t, base: nat, i: nat): BS.uint
+        requires region_index_valid(regions, base, i)
+    {
+        regions[base][i]
+    }
+
+    function wrtie_region(regions: regions_t, base: nat, i: nat, v: BS.uint): regions_t
+        requires region_index_valid(regions, base, i)
+    {
+        var region' := regions[base][i := v];
+        regions[base := region']
+    }
+
+    function as_flat_ptr(base: nat, i: nat): nat
+    {
+        Mul.LemmaMulNonnegative(i, FM.WORD_BYTES);
+        base + i * FM.WORD_BYTES
+    }
+
+    function build_stack_region(mem: FM.mem_t, base: nat, len: nat): seq<BS.uint>
+        requires mem.region_valid(base, len)
+    {
+        seq(len, i requires 0 <= i < len =>
+            mem.flat[as_flat_ptr(base, i)])
+    }
+
+    function build_regions(mem: FM.mem_t): regions_t
+        requires mem.inv()
+    {
+        map base | base in mem.split ::
+            build_stack_region(mem, base, mem.split[base])
+    }
+
+    predicate refines_flat(regions: regions_t, mem: FM.mem_t)
+    {
+        && mem.inv()
+        && regions == build_regions(mem)
+    }
+
+    lemma read_refinement_lemma(regions: regions_t, base: nat, i: nat, mem: FM.mem_t)
+        requires refines_flat(regions, mem)
+        requires region_index_valid(regions, base, i)
+        ensures FM.ptr_aligned(as_flat_ptr(base, i))
+        ensures read_region(regions, base, i) ==
+            mem.read_word(as_flat_ptr(base, i))
+    {
+        assume false;
+    }
+
+    lemma write_refinement_lemma(regions: regions_t, base: nat, i: nat, v: BS.uint, mem: FM.mem_t)
+        requires refines_flat(regions, mem)
+        requires region_index_valid(regions, base, i)
+        ensures FM.ptr_aligned(as_flat_ptr(base, i))
+        ensures refines_flat(wrtie_region(regions, base, i, v),
+            mem.write_word(as_flat_ptr(base, i), v))
+    {
+        assume false;
+    }
+}
+
+abstract module hyper_mem_i(BV: bv_op_s)
+{
+    import Mul
+
+    import RM = regions_mem_i(BV)
+    import FM = RM.FM
+    import BS = FM.BS
+
+    function {:fuel 1} rev_concat(fs: seq<seq<BS.uint>>): seq<BS.uint>
+        decreases |fs|
+    {
+        if |fs| == 0 then
+            []
+        else
+            var index := |fs| - 1;
+            fs[index] + rev_concat(fs[..index])
+    }
+
+    datatype hyper_t = hyper_cons(
+        heap: map<FM.aptr, seq<BS.uint>>,
+        fs: seq<seq<BS.uint>>,
+        free: seq<BS.uint>)
+    {
+        function build_stack_region(): seq<BS.uint>
+        {
+            free + rev_concat(fs)
+        }
+
+        function build_regions(): RM.regions_t
+        {
+            heap[FM.STACK_BOT := build_stack_region()]
+        }
+
+        predicate refines_flat(mem: RM.FM.mem_t)
+        {
+            && mem.inv()
+            && FM.STACK_BOT !in heap
+            && RM.refines_flat(build_regions(), mem)
+        }
+
+        function push_frame_(len: nat): hyper_t
+            requires 0 <= len < |free|
+        {
+            var fs' := fs + [free[len..]];
+            hyper_cons(heap, fs', free[..len])
+        }
+
+        lemma push_refinement_lemma(len: nat)
+            requires 0 <= len < |free|
+            ensures build_stack_region() == 
+                push_frame_(len).build_stack_region()
+        {
+            var stack' := push_frame_(len);
+
+            calc == {
+                stack'.build_stack_region();
+                free[..len] + rev_concat(fs + [free[len..]]);
+                free[..len] + free[len..] + rev_concat(fs);
+                free + rev_concat(fs);
+                build_stack_region();
+            }
+        }
+
+        function pop_frame_(): hyper_t
+            requires |fs| != 0
+        {
+            var index := |fs| - 1;
+            hyper_cons(heap, fs[..index], free + fs[index])
+        }
+
+        lemma pop_refinement_lemma()
+            requires |fs| != 0
+            ensures build_stack_region() == 
+                pop_frame_().build_stack_region()
+        {
+            var stack' := pop_frame_();
+            var index := |fs| - 1;
+
+            calc == {
+                stack'.build_stack_region();
+                free + fs[index] + rev_concat(fs[..index]);
+                free + rev_concat(fs[..index] + [fs[index]]);
+                free + rev_concat(fs);
+                build_stack_region();
+            }
+        }
+
+        predicate valid_frame_index(i: nat)
+        {
+            && |fs| != 0
+            && i < |fs[|fs| - 1]|
+        }
+
+        function write_frame_(i: nat, value: BS.uint): hyper_t
+            requires valid_frame_index(i)
+        {
+            var fi := |fs| - 1;
+            hyper_cons(heap, fs[..fi] + [fs[fi][i := value]], free)
+        }
+
+        lemma write_frame_refinement_lemma(i: nat, value: BS.uint)
+            requires valid_frame_index(i)
+            ensures write_frame_(i, value).build_stack_region() ==
+                build_stack_region()[|free| + i := value];
+        {
+            var stack' := write_frame_(i, value);
+            var fi := |fs| - 1;
+            var fs' := fs[fi][i := value];
+            var si := |free| + i;
+
+            calc == {
+                build_stack_region()[si:= value];
+                (free + rev_concat(fs))[si:= value];
+                free + rev_concat(fs)[i := value];
+                free + rev_concat(fs[..fi] + [fs[fi]])[i := value];
+                free + (fs[fi] + rev_concat(fs[..fi]))[i := value];
+                free + fs[fi][i := value] + rev_concat(fs[..fi]);
+                free + fs' + rev_concat(fs[..fi]);
+                free + rev_concat(fs[..fi] + [fs']);
+                stack'.build_stack_region();
+            }
+        }
+
+        function read_frame_(i: nat): BS.uint
+            requires valid_frame_index(i)
+        {
+            fs[|fs| - 1][i]
+        }
+
+        lemma read_frame_refinement_lemma(i: nat)
+            requires valid_frame_index(i)
+            ensures read_frame_(i) == build_stack_region()[|free| + i];
+        {
+            var fi := |fs| - 1;
+            calc == {
+                build_stack_region()[|free| + i];
+                (free + rev_concat(fs))[|free| + i];
+                rev_concat(fs)[i];
+                rev_concat(fs[..fi] + [fs[fi]])[i];
+                (fs[fi] + rev_concat(fs[..fi]))[i];
+                fs[fi][i];
+            }
+        }
+    }
+
+    datatype iter_t = iter_cons(base_ptr: nat, buff: seq<BS.uint>, index: nat)
+    {
+        function cur_addr(): nat
+        {
+            RM.as_flat_ptr(base_ptr, index)
+        }
+    }
+
+    predicate iter_inv(hyper: hyper_t, iter: iter_t)
+    {
+        var base_ptr := iter.base_ptr;
+        && base_ptr in hyper.heap
+        && iter.index <= |iter.buff|
+        && hyper.heap[base_ptr] == iter.buff
+    }
+
+    predicate iter_safe(hyper: hyper_t, iter: iter_t)
+    {
+        && iter_inv(hyper, iter)
+        && iter.index < |iter.buff|
+    }
+
+// iter read
+
+    function read_iter(hyper: hyper_t, iter: iter_t): (v: BS.uint)
+        requires iter_safe(hyper, iter)
+    {
+        iter.buff[iter.index]
+    }
+
+    function iter_load_next(iter: iter_t, inc: bool): iter_t
+    {
+        iter.(index := if inc then iter.index + 1 else iter.index)
+    }
+
+    lemma read_iter_refinement_lemma(hyper: hyper_t, iter: iter_t, mem: RM.FM.mem_t)
+        requires iter_safe(hyper, iter)
+        requires hyper.refines_flat(mem)
+        ensures FM.ptr_aligned(iter.cur_addr())
+        ensures read_iter(hyper, iter) ==
+            mem.read_word(iter.cur_addr())
+    {
+        var regions := hyper.build_regions();
+        assert iter.buff == regions[iter.base_ptr];
+        RM.read_refinement_lemma(regions, iter.base_ptr, iter.index, mem);
+    }
+
+// iter write
+
+    function write_iter(hyper: hyper_t, iter: iter_t, value: BS.uint):
+        (hyper_t)
+        requires iter_safe(hyper, iter)
+    {
+        var buff' := iter.buff[iter.index := value];
+        hyper.(heap := hyper.heap[iter.base_ptr := buff'])
+    }
+
+    function iter_store_next(iter: iter_t, value: BS.uint, inc: bool): iter_t
+        requires iter.index < |iter.buff|
+    {
+        iter.(index := if inc then iter.index + 1 else iter.index)
+            .(buff := iter.buff[iter.index := value])
+    }
+
+    lemma write_iter_refinement_lemma(hyper: hyper_t, iter: iter_t, value: BS.uint, mem: RM.FM.mem_t)
+        returns (hyper': hyper_t)
+        requires iter_safe(hyper, iter)
+        requires hyper.refines_flat(mem)
+        ensures hyper' == write_iter(hyper, iter, value)
+        ensures FM.ptr_aligned(iter.cur_addr())
+        ensures hyper'.refines_flat(mem.write_word(iter.cur_addr(), value))
+        ensures iter_safe(hyper', iter_store_next(iter, value, false))
+    {
+        var regions := hyper.build_regions();
+        var base := iter.base_ptr;
+        var buff := iter.buff;
+        var index := iter.index;
+        assert buff == regions[base];
+        RM.write_refinement_lemma(regions, base, iter.index, value, mem);
+        hyper' := write_iter(hyper, iter, value);
+        var regions' := hyper'.build_regions();
+        assert regions' == regions[base := buff[index := value]];
+        assert regions' == RM.wrtie_region(regions, base, index, value);
+    }
+
+// stack push
+
+    lemma push_refinement_lemma(hyper: hyper_t, len: nat, mem: RM.FM.mem_t)
+        returns (hyper': hyper_t)
+        requires 0 <= len < |hyper.free|
+        requires hyper.refines_flat(mem)
+        ensures hyper' == hyper.push_frame_(len)
+        ensures hyper'.refines_flat(mem)
+    {
+        // var regions := hyper.build_regions();
+        hyper' := hyper.push_frame_(len);
+        // var regions' := hyper'.build_regions();
+        hyper.push_refinement_lemma(len);
+    }
+
+// stack pop
+
+    lemma pop_refinement_lemma(hyper: hyper_t, len: nat, mem: RM.FM.mem_t)
+        returns (hyper': hyper_t)
+        requires |hyper.fs| != 0
+        requires hyper.refines_flat(mem)
+        ensures hyper' == hyper.pop_frame_()
+        ensures hyper'.refines_flat(mem)
+    {
+        // var regions := hyper.build_regions();
+        hyper' := hyper.pop_frame_();
+        // var regions' := hyper'.build_regions();
+        hyper.pop_refinement_lemma();
+    }
+
+// stack read
+
+    lemma read_frame_refinement_lemma(hyper: hyper_t, i: nat, mem: RM.FM.mem_t)
+        requires hyper.valid_frame_index(i)
+        requires hyper.refines_flat(mem)
+        ensures FM.ptr_aligned(RM.as_flat_ptr(FM.STACK_BOT, i + |hyper.free|))
+        ensures hyper.read_frame_(i) ==
+            mem.read_word(RM.as_flat_ptr(FM.STACK_BOT, i + |hyper.free|))
+    {
+        var regions := hyper.build_regions();
+        var base := FM.STACK_BOT;
+        hyper.read_frame_refinement_lemma(i);
+        var j := |hyper.free| + i;
+        RM.read_refinement_lemma(regions, base, j, mem);
+    }
+
+// stack write
+
+    lemma write_frame_refinement_lemma(hyper: hyper_t, i: nat, value: BS.uint, mem: RM.FM.mem_t)
+        returns (hyper': hyper_t)
+        requires hyper.valid_frame_index(i)
+        requires hyper.refines_flat(mem)
+        ensures hyper' == hyper.write_frame_(i, value)
+        ensures FM.ptr_aligned(RM.as_flat_ptr(FM.STACK_BOT, i + |hyper.free|))
+        ensures hyper'.refines_flat(
+            mem.write_word(RM.as_flat_ptr(FM.STACK_BOT, i + |hyper.free|), value))
+    {
+        hyper' := hyper.write_frame_(i, value);
+        var regions := hyper.build_regions();
+        var regions' := hyper'.build_regions();
+        var base := FM.STACK_BOT;
+        hyper.write_frame_refinement_lemma(i, value);
+        var j := |hyper.free| + i;
+        var stack' := regions[base][j := value];
+        assert regions' == regions[base := stack'];
+        assert regions' == RM.wrtie_region(regions, base, j, value);
+        RM.write_refinement_lemma(regions, base, j, value, mem);
+    }
+}
+
+// abstract module test {
+//     import opened integers
+//     import BV32 = bv32_op_s
+//     import BV256 = bv256_op_s
+
+//     import HM = hyper_mem_i(BV32)
+//     import RM = HM.RM
+//     import FM = RM.FM
+
+//     // import FM = HM.FM
+
+//     import IT32 = recast_iter_i(BV32, BV32)
+//     import IT256 = recast_iter_i(BV32, BV256)
+
+//     function read_iter32(hyper: HM.hyper_t, iter: IT32.iter_t): uint32
+//         requires IT32.iter_safe(hyper, iter);
+//     {
+//         IT32.uint_bound_lemma();
+//         IT32.read_iter(hyper, iter)
+//     }
+
+//     lemma read_iter32_refinement_lemma(hyper: HM.hyper_t, iter: IT32.iter_t, mem:   FM.mem_t)
+//         requires mem.inv()
+//         requires hyper.refines_flat(mem)
+//         // ensures 
+
+//     function read_iter256(hyper: HM.hyper_t, iter: IT256.iter_t): uint256
+//         requires IT256.iter_safe(hyper, iter);
+//     {
+//         IT256.uint_bound_lemma();
+//         IT256.read_iter(hyper, iter)
+//     }
+
+// }
